rocq-osiris/interp/O2E.ml
@@ -140,6 +140,7 @@ let rec expr : O.expr -> E.expr = function
   | ERef e -> ERef (expr e)
   | ELoad e -> ELoad (expr e)
   | EStore (e1, e2) -> EStore (expr e1, expr e2)
+  | ECAS (e1, e2, e3) -> ECAS (expr e1, expr e2, expr e3)
   | EFork (e1, e2) -> EFork (expr e1, expr e2)
   | EJoin e -> EJoin (expr e)
 
