rocq-osiris/theories/semantics/run.v
@@ -49,7 +49,7 @@ Fixpoint confluent_step {A E} (σ : store) (m : micro A E) : option (config A E)
   (* Final micros do not step *)
   | Ret _ | Throw _ | Crash => None
   (* Most side effects are not confluent *)
-  | Stop (CFlip | CLoad | CStore | CPerf | CResume | CWrap | CFork | CJoin) _ _ => None
+  | Stop (CFlip | CLoad | CStore | CCAS | CPerf | CResume | CWrap | CFork | CJoin) _ _ => None
   (* [CEval], [CLoop], [CAlloc], [Handle] have only one way to reduce *)
   | Stop CEval (η, e) k => Some (σ, try2 (pre_eval η e) k)
   | Stop CLoop (η, x, i1, i2, e) k => Some (σ, try2 (loop η x i1 i2 e) k)
@@ -127,6 +127,7 @@ Fixpoint stepto {A E} (σ : store) (m : micro A E) {struct m} : step_result A E 
   (* [Stop] cases involving the store or flips typically break confluence *)
   | Stop CLoad l k => Step [step_load σ l k]
   | Stop CStore (l, v') k => Step [step_store σ l v' k]
+  | Stop CCAS (l, seen, v') k => Step [step_cas σ l seen v' k]
   | Stop CResume (l, o) k => Step [step_resume σ l o k]
   | Stop CWrap (true, l, η, bs) k => Step [step_wrap σ l η bs (fresh (dom σ)) k]
   | Stop CWrap (false, l, η, bs) k => Step [step_shallow_wrap σ l η bs (fresh (dom σ)) k]
@@ -363,6 +364,7 @@ Fixpoint string_of_expr (e : expr) : string :=
   | ERef e => "ERef(" ++ string_of_expr e ++ ")"
   | ELoad e => "ELoad(" ++ string_of_expr e ++ ")"
   | EStore e1 e2 => "EStore(" ++ string_of_expr e1 ++ ", " ++ string_of_expr e2 ++ ")"
+  | ECAS e1 e2 e3 => "ECAS(" ++ string_of_expr e1 ++ ", " ++ string_of_expr e2 ++ ", " ++ string_of_expr e3 ++ ")"
   | EFork e1 e2 => "EFork(" ++ string_of_expr e1 ++ ", " ++ string_of_expr e2 ++ ")"
   | EJoin e => "EFork(" ++ string_of_expr e ++ ")"
   end
@@ -443,6 +445,7 @@ Definition string_of_code {X Y Z} (c : code X Y Z) : string :=
   | CAllocn => "CAllocn"
   | CLoad => "CLoad"
   | CStore => "CStore"
+  | CCAS => "CCAS"
   | CPerf => "CPerf"
   | CResume => "CResume"
   | CWrap => "CWrap"
@@ -470,6 +473,7 @@ Fixpoint string_of_micro {A E} (ppa : A → string) (ppe : E → string) (m : mi
   | Stop CAllocn vs k => "Stop(CAlloc" ++ ", [" ++ String.concat "; " (map string_of_val vs) ++ "]" ++ ", <cont>)"
   | Stop CLoad loc k => "Stop(CLoad" ++ ", " ++ string_of_Z loc.(address) ++ ", <cont>)"
   | Stop CStore (loc, v) k => "Stop(CStore" ++ ", " ++ string_of_Z loc.(address) ++ ", " ++ string_of_val v ++ ", <cont>)"
+  | Stop CCAS (loc, seen, v) k => "Stop(CCAS" ++ ", " ++ string_of_Z loc.(address) ++ ", " ++ string_of_val seen ++ ", " ++ string_of_val v ++ ", <cont>)"
   | Stop CPerf v k => "Stop(CPerf" ++ ", " ++ string_of_val v ++ ", <cont>)"
   | Stop CResume (loc, o2) k => "Stop(CResume" ++ ", " ++ string_of_Z loc.(address) ++ ", " ++ string_of_outcome2 o2 ++ ", <cont>)"
   | Stop CWrap (d, loc, η, h) k => "Stop(CWrap" ++ ", " ++ string_of_bool d ++ ", " ++ string_of_Z loc.(address) ++ "<env>, <handler>" ++ ", <cont>)"
